library/init/util.lean
@@ -13,5 +13,5 @@ def dbgTrace {α : Type u} (s : String) (f : Unit → α) : α :=
 f ()
 
 @[extern cpp inline "lean::dbg_sleep(#2, #3)"]
-def dbgSleep {α : Type u} (ms : Uint32) (f : Unit → α) : α :=
+def dbgSleep {α : Type u} (ms : UInt32) (f : Unit → α) : α :=
 f ()
